pixelState.v
@@ -1,5 +1,5 @@
-Require Import graphicsTypeClass.
-
+Require Export  graphicsTypeClass.
+Module pix_prop := FMapFacts.Properties pix.
 Record pixelState :=
   mkPState
   {
@@ -13,13 +13,76 @@ Next Obligation.
 
 (*Our usefule instance that still needs some additions but includes a 
   way to make an initial state update the screen size and draw a pixel*)
+Definition eq s s' : Prop :=
+  pix.Equal (screen_state s) (screen_state s').
+
+Lemma eq_refl : forall s, eq s s.
+Proof.
+  intros.
+  unfold eq.
+  destruct s.
+  simpl.
+  constructor.
+Qed.
+
+Lemma eq_sym : forall x y , eq x y -> eq y x.
+Proof.
+  unfold eq. unfold pix.Equal.
+  intros.
+  auto.
+Qed.
+
+
+Lemma eq_trans : forall x y z , eq x y -> eq y z -> eq x z.
+Proof.
+  unfold eq.
+  intros; simpl.
+  destruct x, y, z.
+  unfold pix.Equal in *.
+  intros.
+  rewrite H.
+  rewrite H0.
+  auto.
+Qed.
+
+Definition draw_pixel := (fun s p c => mkPState (update p c (screen_state s)) (screen_size s)).
+
+
+Lemma  pix_ok : forall (p1 p2 : point) (c1 c2 : color) t,
+             p1 <> p2 ->
+             eq (draw_pixel (draw_pixel t p2 c1) p1 c2)
+               (draw_pixel (draw_pixel t p1 c2) p2 c1).
+Proof.
+  intros.
+  unfold eq.
+  simpl.
+  unfold update.
+  unfold pix.Equal.
+  intros .
+  do 4 rewrite pix_prop.F.add_o.
+  unfold not in H.
+  case_eq (pix.E.eq_dec p2 y);
+    case_eq (pix.E.eq_dec p1 y); auto.
+  intros.
+  destruct a, a0.
+  destruct p1,p2,y.
+  simpl in *.
+  subst.
+  destruct H; auto.
+Qed.
+
 Instance pixelMap_graphics_prims : graphics_prims pixelState :=
-  mkGraphicsPrims
-    pixelState
+  mkGraphicsPrims pixelState
     (init)
     (fun s p => mkPState (screen_state s) p)
-    (fun s p c => mkPState (update p c (screen_state s)) (screen_size s)).
+    draw_pixel
+    eq
+    eq_refl
+    eq_sym
+    eq_trans
+    pix_ok.
 
+Open Scope Z_scope.
 Definition prog1 : g_com :=
    lineto (1,2) (1,20) Red.
   (* draw_rect (1,2) (3,4) Red. *)
@@ -32,4 +95,3 @@ Fixpoint toListPair (l : list (pix.key * color)) : list (pix.key):=
   end.
 
 Definition hi := (pix.elements (screen_state (interp (init_state tt) prog1))).
-Compute hi.
