d_and.v
@@ -1,0 +1,44 @@
+Open Scope nat_scope.
+Ltac solve_by_inverts n :=
+  match goal with | H : ?T |- _ => 
+  match type of T with Prop =>
+    solve [ 
+      inversion H; try reflexivity;
+      match n with S (S (?n')) => subst; solve_by_inverts (S n') end ]
+  end end.
+
+Ltac solve_by_invert :=
+  solve_by_inverts 3.
+
+Set Implicit Arguments.
+
+
+Ltac d_all n :=
+  try intros; repeat subst; auto;
+    match n with
+    | 0 => (  repeat simpl in *; match goal with
+              | H : _/\ _  |- _ =>
+                destruct H; eauto; try solve_by_inverts 1; subst;
+                try d_all 0
+              | H : exists _, _|- _ => destruct H;
+                           try solve_by_inverts 2; auto; try d_all 0
+              | H : _ |- ~ _ => unfold not in *; simpl in *;
+                                intros; auto; try solve_by_inverts 1;
+                                try d_all 0
+              | H :~ _ |-  _ => unfold not in H; simpl in *; intros;
+                               try solve_by_inverts 1; auto; try d_all 0
+              | _ => auto; try solve_by_inverts 1; try d_all 1
+              end)
+    | 1 =>  match goal with
+                | H : _ \/ _ |- _ => destruct H; auto;
+                                     solve_by_inverts 1; try d_all 0
+                | _ => intuition; try solve_by_inverts 1
+                end
+  end.
+
+Ltac d_and :=
+  d_all 0.
+Ltac d_or :=
+  d_all 1.
+Ltac uncomp := 
+ d_all 2.
